Cleanup, add simpler theorems

src/LogRel.v
@@ -1,6 +1,4 @@
-Require Export SubstSemantics.
-Export Relations.Relations.
-Export Classes.RelationClasses.
+Require Export Scoping.
 
 Import ListNotations.
 
@@ -15,36 +13,6 @@ Proof.
   * intro. intros. unfold R' in *. destruct H1, H2. split.
     - eapply H0; eauto.
     - eapply H0; eauto.
-Qed.
-
-Definition is_value_b (e : Exp) : bool :=
-match e with
-| ELit _ | EFun _ _ | ERecFun _ _ _ => true
-| _ => false
-end.
-
-Theorem is_value_equiv :
-  forall v, is_value v <-> is_value_b v = true.
-Proof.
-  split.
-  {
-    destruct v; intros; inversion H; auto.
-  }
-  {
-    destruct v; intros; simpl in H; try congruence; constructor.
-  }
-Qed.
-
-Theorem is_value_nequiv :
-  forall v, ~ is_value v <-> is_value_b v = false.
-Proof.
-  split.
-  {
-    intros; destruct v; auto; exfalso; apply H; constructor.
-  }
-  {
-    intros; destruct v; simpl in H; try congruence; intro; inversion H0.
-  }
 Qed.
 
 (* I think this definition is not suitable for equivalence:
@@ -63,46 +31,6 @@ Definition exp_rel (n : nat)
     (Vrel m Hmn v1 v2 /\ (* maybe -> ? *)
      eval m e1 = Res v1) -> (exists clock, eval clock e2 = Res v2)
 . *)
-Reserved Notation "'EXP' Γ ⊢ e"
-         (at level 69, no associativity).
-
-Reserved Notation "'VAL' Γ ⊢ v"
-         (at level 69, no associativity).
-Inductive ExpScoped (l : list VarFunId) : Exp -> Prop :=
-| scoped_var v : In (inl v) l -> EXP l ⊢ EVar v
-| scoped_funid f : In (inr f) l -> EXP l ⊢ EFunId f
-| scoped_app exp vals : 
-  EXP l ⊢ exp ->
-  (forall i, i < length vals -> EXP l ⊢ nth i vals (ELit 0))
-->
-  EXP l ⊢ EApp exp vals
-| scoped_let v e1 e2 :
-  EXP l ⊢ e1 -> EXP (l ++ [inl v]) ⊢ e2 
-->
-  EXP l ⊢ ELet v e1 e2
-| scoped_letrec f vl b e :
-  EXP (l ++ [inr f] ++ map inl vl) ⊢ b -> EXP (l ++ [inr f]) ⊢ e
-->
-  EXP l ⊢ ELetRec f vl b e
-| scoped_plus e1 e2 :
-  EXP l ⊢ e1 -> EXP l ⊢ e2
-->
-  EXP l ⊢ EPlus e1 e2
-| scoped_if e1 e2 e3 :
-  EXP l ⊢ e1 -> EXP l ⊢ e2 -> EXP l ⊢ e3
-->
-  EXP l ⊢ EIf e1 e2 e3
-| scoped_val v :
-  VAL l ⊢ v -> EXP l ⊢ v
-with ValScoped (l : list VarFunId) : Exp -> Prop :=
-| scoped_lit lit : VAL l ⊢ ELit lit
-| scoped_fun vl e : EXP (l ++ (map inl vl)) ⊢ e -> VAL l ⊢ EFun vl e
-| scoped_recfun f vl e : EXP (l ++ [inr f] ++ (map inl vl)) ⊢ e -> VAL l ⊢ ERecFun f vl e
-where "'EXP' Γ ⊢ e" := (ExpScoped Γ e)
-and "'VAL' Γ ⊢ e" := (ValScoped Γ e).
-
-Notation "'EXPCLOSED' e" := (EXP [] ⊢ e) (at level 5).
-Notation "'VALCLOSED' v" := (VAL [] ⊢ v) (at level 5).
 
 Definition exp_rel (n : nat)
                    (Vrel : forall m, m <= n -> Exp -> Exp -> Prop)
@@ -375,10 +303,6 @@ Definition subscoped (l l' : list VarFunId) (ξ : VarFunId -> Exp) : Prop :=
 Notation "'SUBSCOPE' Γ ⊢ ξ :: Γ'" := (subscoped Γ Γ' ξ) (at level 69, ξ at level 99, no associativity).
 *)
 
-Definition subscoped (l' : list VarFunId) (vals : list Exp) : Prop :=
-  forall i, i < length vals -> ValScoped l' (nth i vals (ELit 0))
-.
-
 (* Def: closed values are related *)
 Definition Grel (n : nat) (vals1 vals2 : list Exp) : Prop :=
   subscoped [] vals1 /\ subscoped [] vals2 /\ length vals1 = length vals2 /\
@@ -435,511 +359,77 @@ Proof.
   unfold Grel; intros; intuition. eapply Grel_downclosed_helper; eauto.
 Qed.
 
-Corollary app_not_in {T : Type} : forall (x:T) (l1 l2 : list T),
-  ~In x l1 -> ~In x l2 -> ~In x (l1 ++ l2).
+Definition Vrel_open (Γ : list VarFunId) (e1 e2 : Exp) :=
+  forall n vals1 vals2,
+  length vals1 = length Γ -> length vals2 = length Γ -> Grel n vals1 vals2
+->
+  Vrel n (subst_list Γ vals1 e1) (subst_list Γ vals2 e2).
+
+Definition Erel_open (Γ : list VarFunId) (e1 e2 : Exp) :=
+  forall n vals1 vals2,
+  length vals1 = length Γ -> length vals2 = length Γ -> Grel n vals1 vals2
+->
+  Erel n (subst_list Γ vals1 e1) (subst_list Γ vals2 e2).
+
+Lemma subscoped_to_vrel vals :
+  subscoped [] vals ->
+  list_biforall (Vrel 0) vals vals.
+Proof.
+  induction vals; intros; constructor.
+  - rewrite Vrel_Fix_eq. specialize (H 0 (Nat.lt_0_succ _)). simpl in H.
+    unfold Vrel_rec. destruct H.
+    + intuition. all: constructor.
+    + intuition. 1-2: constructor; auto. break_match_goal. 2: congruence.
+      intros. inversion Hmn.
+    + intuition. 1-2: constructor; auto. break_match_goal. 2: congruence.
+      intros. inversion Hmn.
+  - apply IHvals. intro. intros. apply (H (S i)). simpl. lia.
+Qed.
+
+Lemma Erel_open_closed : forall {Γ e1 e2},
+    Erel_open Γ e1 e2 ->
+    forall vals, subscoped [] vals -> length vals = length Γ ->
+              EXPCLOSED (subst_list Γ vals e1) /\ EXPCLOSED (subst_list Γ vals e2).
 Proof.
   intros.
-  intro. eapply in_app_or in H1. destruct H1; contradiction.
+  apply @Erel_closed with (n:=0).
+  apply H; auto.
+  unfold Grel.
+  intuition idtac.
+  apply subscoped_to_vrel. auto.
 Qed.
 
-Theorem in_list_sound : forall l e, in_list e l = true <-> In e l.
+Lemma Erel_open_scope : forall {Γ e1 e2},
+    Erel_open Γ e1 e2 ->
+    EXP Γ ⊢ e1 /\ EXP Γ ⊢ e2.
 Proof.
-  induction l; intros.
-  * split; intros; inversion H.
-  * split; intros.
-    - simpl in H. break_match_hyp.
-      + apply eqb_eq in Heqb. simpl. left. auto.
-      + apply eqb_neq in Heqb. simpl. right. apply IHl. auto.
-    - destruct (eqb e a) eqn:P.
-      + apply eqb_eq in P. subst. simpl. rewrite eqb_refl. auto.
-      + simpl. rewrite P. apply IHl. inversion H.
-        ** apply eqb_neq in P. congruence.
-        ** auto.
-Qed.
-
-Hint Resolve in_list_sound.
-
-Theorem not_in_list_sound : forall l e, in_list e l = false <-> ~In e l.
-Proof.
-  induction l; intros.
-  * split; intros. intro. inversion H0. reflexivity.
-  * split; intros.
-    - simpl in H. break_match_hyp.
-      + inversion H.
-      + apply eqb_neq in Heqb. simpl. intro. inversion H0. symmetry in H1. contradiction.
-        eapply IHl; eauto.
-    - simpl. break_match_goal.
-      apply eqb_eq in Heqb. subst. exfalso. apply H. intuition.
-      apply eqb_neq in Heqb. eapply IHl. apply not_in_cons in H. destruct H. auto.
-Qed.
-
-Hint Resolve not_in_list_sound.
-
-Definition Injective {A B} (f : A->B) :=
- forall x y, f x = f y -> x = y.
-
-Theorem map_not_in {T T' : Type} : forall (l : list T) (x: T) (f : T -> T'),
-  Injective f -> ~In x l -> ~In (f x) (map f l).
-Proof.
-  induction l; intros; intro.
-  * inversion H1.
-  * inversion H1.
-    - apply H in H2. subst. apply H0. intuition.
-    - eapply IHl; eauto. apply not_in_cons in H0. destruct H0. auto.
-Qed.
-
-Scheme ValScoped_ind2 := Induction for ValScoped Sort Prop
-  with ExpScoped_ind2 := Induction for ExpScoped Sort Prop.
-Combined Scheme scoped_ind from ValScoped_ind2, ExpScoped_ind2.
-Check scoped_ind.
-
-Theorem scoped_ignores_sub_helper vals : forall x l v,
-  (forall i : nat,
-     i < Datatypes.length vals ->
-     forall (x : ExpEnv.Var) (v : Exp),
-     ~ In (@inl Var FunctionIdentifier x) l -> varsubst x v (nth i vals (ELit 0)) = nth i vals (ELit 0)) ->
-  ~ In (inl x) l ->
-  (map (varsubst x v) vals) = vals.
-Proof.
-  induction vals; intros.
-  * reflexivity.
-  * simpl. epose (H 0 _ _ _ H0). simpl in e. rewrite e.
-    erewrite IHvals; eauto. intros. eapply (H (S i)). simpl. lia. auto.
-Unshelve. simpl. lia.
-Qed.
-
-Theorem scoped_ignores_sub : forall Γ,
-  (forall e, VAL Γ ⊢ e -> forall x v, ~ In (inl x) Γ -> varsubst x v e = e) /\
-  (forall e, EXP Γ ⊢ e -> forall x v, ~ In (inl x) Γ -> varsubst x v e = e).
-Proof.
-  apply scoped_ind.
-  * intros. reflexivity.
-  * intros. simpl. break_match_goal; auto. rewrite H; auto.
-    apply app_not_in; auto. intuition. apply not_in_list_sound in Heqb.
-    eapply map_not_in in Heqb. exact (Heqb H1). intro. intros. inversion H2. auto.
-  * intros. simpl. break_match_goal; auto. rewrite H; auto.
-    repeat apply app_not_in; auto. intro. inversion H1; try congruence. contradiction.
-    apply not_in_list_sound in Heqb.
-    eapply map_not_in in Heqb. intro. exact (Heqb H1). intro. intros. inversion H1. auto.
-  * intros. simpl. break_match_goal; auto. apply eqb_eq in Heqb. subst. contradiction.
-  * intros. simpl. auto.
-  * intros. simpl. rewrite H; auto. erewrite scoped_ignores_sub_helper; eauto.
-  * intros. simpl. break_match_goal.
-    - rewrite H; auto.
-    - rewrite H, H0; auto. eapply app_not_in; auto.
-      intro. inversion H2. 2: contradiction. apply eqb_neq in Heqb. inversion H3. congruence.
-  * intros. simpl. break_match_goal; auto.
-    - rewrite H0; auto. eapply app_not_in; auto.
-      intro. inversion H2; try contradiction; try congruence.
-    - rewrite H, H0. auto.
-      + eapply app_not_in; auto.
-      intro. inversion H2; try contradiction; try congruence.
-      + apply app_not_in; auto. Search In map. eapply app_not_in. intro.
-        inversion H2; try contradiction; try congruence.
-        apply not_in_list_sound in Heqb0.
-        eapply map_not_in in Heqb0. intro. exact (Heqb0 H2).
-        intro. intros. inversion H2. auto.
-  * intros. simpl. rewrite H, H0; auto.
-  * intros. simpl. rewrite H, H0, H1; auto.
-  * intros. eapply H; eauto.
-Qed.
-
-Corollary eclosed_ignores_sub :
-  forall e x v,
-  EXPCLOSED e -> varsubst x v e = e.
-Proof.
-  intros. eapply scoped_ignores_sub with (Γ := []). auto. intuition.
-Qed.
-
-Corollary vclosed_ignores_sub :
-  forall e x v,
-  VALCLOSED e -> varsubst x v e = e.
-Proof.
-  intros. pose (scoped_ignores_sub []). destruct a. apply H0. auto. intuition.
-Qed.
-
-Theorem scoped_ignores_funsub_helper vals : forall x l v,
-  (forall i : nat,
-     i < Datatypes.length vals ->
-     forall (x : FunctionIdentifier) (v : Exp),
-     ~ In (@inr Var FunctionIdentifier x) l -> funsubst x v (nth i vals (ELit 0)) = nth i vals (ELit 0)) ->
-  ~ In (inr x) l ->
-  (map (funsubst x v) vals) = vals.
-Proof.
-  induction vals; intros.
-  * reflexivity.
-  * simpl. epose (H 0 _ _ _ H0). simpl in e. rewrite e.
-    erewrite IHvals; eauto. intros. eapply (H (S i)). simpl. lia. auto.
-Unshelve. simpl. lia.
-Qed.
-
-Lemma inr_inl_map x l:
-  In (@inr Var FunctionIdentifier x) (map inl l) -> False.
-Proof.
-  induction l; intros; inversion H.
-  inversion H0. apply IHl. auto.
-Qed.
-
-Theorem scoped_ignores_funsub : forall Γ,
-  (forall e, VAL Γ ⊢ e -> forall x v, ~ In (inr x) Γ -> funsubst x v e = e) /\
-  (forall e, EXP Γ ⊢ e -> forall x v, ~ In (inr x) Γ -> funsubst x v e = e).
-Proof.
-  apply scoped_ind.
-  * intros. reflexivity.
-  * intros. simpl. rewrite H; auto.
-    apply app_not_in; auto. intuition.
-    apply inr_inl_map in H1. auto.
-  * intros. simpl. break_match_goal; auto.
-    rewrite H; auto.
-    repeat apply app_not_in; auto.
-    intro. inversion H1. inversion H2. apply funid_eqb_neq in Heqb. 1-2: contradiction.
-    exact (inr_inl_map x vl).
-  * intros. simpl. auto.
-  * intros. simpl. break_match_goal; auto. apply funid_eqb_eq in Heqb. subst. contradiction.
-  * intros. simpl. rewrite H; auto. erewrite scoped_ignores_funsub_helper; eauto.
-  * intros. simpl. rewrite H, H0; auto. eapply app_not_in; auto.
-      intro. inversion H2. 2: contradiction. inversion H3.
-  * intros. simpl. break_match_goal; auto.
-    - rewrite H, H0. auto.
-      + eapply app_not_in; auto.
-        intro. inversion H2. 2: contradiction. inversion H3. subst.
-        pose (funid_eqb_refl x). rewrite e5 in Heqb0. inversion Heqb0.
-      + apply app_not_in; auto. eapply app_not_in.
-        intro. inversion H2; inversion H3. subst. apply funid_eqb_neq in Heqb0. congruence.
-        exact (inr_inl_map x vl).
-  * intros. simpl. rewrite H, H0; auto.
-  * intros. simpl. rewrite H, H0, H1; auto.
-  * intros. eapply H; eauto.
-Qed.
-
-Corollary eclosed_ignores_funsub :
-  forall e x v,
-  EXPCLOSED e -> funsubst x v e = e.
-Proof.
-  intros. eapply scoped_ignores_funsub with (Γ := []). auto. intuition.
-Qed.
-
-Corollary vclosed_ignores_funsub :
-  forall e x v,
-  VALCLOSED e -> funsubst x v e = e.
-Proof.
-  intros. pose (scoped_ignores_funsub []). destruct a. apply H0. auto. intuition.
+  intros.
+  pose proof (Erel_open_closed H).
+  split;
+  eapply sub_implies_scope_exp;
+  intros;
+  apply H0; auto.
 Qed.
 
 
 
-(** Closing substitution *)
-Definition subst (v' : VarFunId) (what wher : Exp) : Exp :=
-  match v' with
-  | inl v => varsubst v what wher
-  | inr f => funsubst f what wher
-  end.
 
-Lemma subst_ignores_var : forall v v' val, inl v <> v' -> subst v' val (EVar v) = EVar v.
-Proof.
-  intros. unfold subst. simpl. destruct v'; auto.
-  break_match_goal; auto. apply eqb_eq in Heqb. subst. congruence.
-Qed.
 
-Lemma subst_ignores_funid : forall v v' val, inr v <> v' -> subst v' val (EFunId v) = EFunId v.
-Proof.
-  intros. unfold subst. simpl. destruct v'; auto.
-  break_match_goal; auto. apply funid_eqb_eq in Heqb. subst. congruence.
-Qed.
 
-Definition subst_list (l : list VarFunId) (es : list Exp) (e : Exp) : Exp :=
-  fold_left (fun acc '(v, val) => subst v val acc) (combine l es) e.
 
-Check scoped_ind.
-Check Exp_ind2.
 
-Theorem scope_duplicate :
-  forall e Γ v, In v Γ -> EXP (v :: Γ) ⊢ e -> EXP Γ ⊢ e.
-Proof.
-  einduction e using Exp_ind2 with 
-      (Q := fun l => list_forall (fun e => forall Γ v, In v Γ -> EXP (v :: Γ) ⊢ e -> EXP Γ ⊢ e) l); intros.
-  * constructor. constructor.
-  * inversion H0. subst. 2: inversion H1. constructor. inversion H2; subst; auto.
-  * inversion H0. subst. 2: inversion H1. constructor. inversion H2; subst; auto.
-  * constructor. constructor. inversion H0. inversion H1. subst.
-    rewrite <- app_comm_cons in H4. apply IHe0 in H4; auto. apply in_or_app. left. auto.
-  * constructor. constructor. inversion H0. inversion H1. subst.
-    rewrite <- app_comm_cons in H4. apply IHe0 in H4; auto. apply in_or_app. left. auto.
-  * inversion H0. 2: inversion H1. subst. rewrite indexed_to_forall in IHe1.
-    constructor.
-    - eapply IHe0; eauto.
-    - intros. eapply IHe1; eauto.
-  * inversion H0. 2: inversion H1. subst. constructor.
-    - eapply IHe0_1. exact H. auto.
-    - rewrite <- app_comm_cons in H5. eapply IHe0_2. 2: exact H5.
-      apply in_or_app. left. auto.
-  * inversion H0. 2: inversion H1. subst. constructor.
-    - eapply IHe0_1. apply in_or_app. left. eauto. rewrite <- app_comm_cons in H3. auto.
-    - eapply IHe0_2. apply in_or_app. left. eauto. rewrite <- app_comm_cons in H6. auto.
-  * inversion H0. 2: inversion H1. subst. constructor.
-    - eapply IHe0_1; eauto.
-    - eapply IHe0_2; eauto.
-  * inversion H0. 2: inversion H1. subst. constructor.
-    - eapply IHe0_1; eauto.
-    - eapply IHe0_2; eauto.
-    - eapply IHe0_3; eauto.
-  * constructor; eauto.
-  * constructor.
-Qed.
 
-Require Import Sorting.Permutation.
 
-Theorem perm_scoped : forall Γ,
-  (forall e, VAL Γ ⊢ e -> forall Γ', Permutation Γ Γ' -> VAL Γ' ⊢ e) /\
-  (forall e, EXP Γ ⊢ e -> forall Γ', Permutation Γ Γ' ->  EXP Γ' ⊢ e).
-Proof.
-  apply scoped_ind; intros.
-  * constructor.
-  * constructor. apply H. apply Permutation_app; intuition.
-  * constructor. apply H. apply Permutation_app; intuition.
-  * constructor. eapply Permutation_in. exact H. auto.
-  * constructor. eapply Permutation_in. exact H. auto.
-  * constructor; intuition.
-  * constructor; intuition. apply H0.
-    apply Permutation_app; intuition.
-  * constructor. apply H. apply Permutation_app; intuition.
-    apply H0. apply Permutation_app; intuition.
-  * constructor; intuition.
-  * constructor; intuition.
-  * constructor; intuition.
-Qed.
 
-Theorem scope_ext : forall Γ,
-  (forall e, VAL Γ ⊢ e -> forall v, VAL v::Γ ⊢ e) /\
-  forall e, EXP Γ ⊢ e -> forall v, EXP v::Γ ⊢ e.
-Proof.
-  apply scoped_ind.
-  * intros. constructor.
-  * intros. constructor. apply H.
-  * intros. constructor. apply H.
-  * intros. constructor. constructor 2. auto.
-  * intros. constructor. constructor 2. auto.
-  * intros. constructor. apply H. intros. eapply H0. auto.
-  * intros. constructor. apply H. apply H0.
-  * intros. constructor. apply H. apply H0.
-  * intros. constructor. apply H. apply H0.
-  * intros. constructor. apply H. apply H0. apply H1.
-  * intros. constructor. apply H.
-Qed.
 
-Theorem app_cons_swap {T : Type} : forall (l l' : list T) (a : T),
-  l ++ a::l' = l ++ [a] ++ l'.
-Proof.
-  firstorder.
-Qed.
 
-Corollary scope_ext_app : forall l Γ,
-  (forall e, VAL Γ ⊢ e -> VAL Γ ++ l ⊢ e) /\
-  forall e, EXP Γ ⊢ e -> EXP Γ ++ l ⊢ e.
-Proof.
- induction l; intros.
- * repeat rewrite app_nil_r. split; intros; auto.
- * rewrite app_cons_swap. pose (scope_ext Γ). specialize (IHl (Γ ++ [a])).
-   destruct IHl, a0. split; intros.
-   - specialize (H1 e H3 a). eapply perm_scoped in H1. rewrite app_assoc.
-     apply H. exact H1. apply Permutation_cons_append.
-   - specialize (H2 e H3 a). eapply perm_scoped in H2. rewrite app_assoc.
-     apply H0. exact H2. apply Permutation_cons_append.
-Qed.
 
-Theorem scope_sub v : forall e,
-  (forall Γ, VAL (inl v::Γ) ⊢ e -> forall val, VAL Γ ⊢ val -> VAL Γ ⊢ (varsubst v val e)) /\
-  (forall Γ, EXP (inl v::Γ) ⊢ e -> forall val, EXP Γ ⊢ val -> EXP Γ ⊢ (varsubst v val e)).
-Proof.
-  einduction e using Exp_ind2 with 
-  (Q := fun l => list_forall (fun e => (forall Γ, VAL (inl v::Γ) ⊢ e -> forall val, VAL Γ ⊢ val -> VAL Γ ⊢ (varsubst v val e)) /\
-  (forall Γ, EXP (inl v::Γ) ⊢ e -> forall val, EXP Γ ⊢ val -> EXP Γ ⊢ (varsubst v val e))) l); intros.
-  * split; intros; simpl; constructor. constructor.
-  * split; intros. inversion H.
-    inversion H. 2: inversion H1.
-    subst. simpl. break_match_goal.
-    - apply eqb_eq in Heqb. subst. simpl. auto.
-    - apply eqb_neq in Heqb. inversion H2. inversion H1. congruence.
-      constructor. auto.
-  * split; intros. inversion H.
-    inversion H. 2: inversion H1.
-    subst. simpl. inversion H2. inversion H1. constructor. auto.
-  * split; intros; inversion H; subst; simpl; break_match_goal; constructor.
-    3-4: constructor.
-    - apply in_list_sound in Heqb. rewrite <- app_comm_cons in H2.
-      eapply scope_duplicate in H2; auto. apply in_app_iff. right. apply in_map. auto.
-    - apply IHe0. rewrite <- app_comm_cons in H2. auto.
-      eapply scope_ext_app. constructor. auto.
-    - apply in_list_sound in Heqb. inversion H1; subst. 
-      rewrite <- app_comm_cons in H3.
-      eapply scope_duplicate in H3; auto. apply in_app_iff. right. apply in_map. auto.
-    - inversion H1. subst. apply IHe0. rewrite app_comm_cons. auto.
-      eapply scope_ext_app. auto.
-  * split; intros; inversion H; subst; simpl; break_match_goal; constructor.
-    3-4: constructor.
-    - apply in_list_sound in Heqb. rewrite <- app_comm_cons in H2.
-      eapply scope_duplicate in H2; auto. apply in_app_iff. right.
-      apply in_app_iff. right. apply in_map. auto.
-    - apply IHe0. rewrite <- app_comm_cons in H2. auto.
-      eapply scope_ext_app. constructor. auto.
-    - apply in_list_sound in Heqb. inversion H1; subst. 
-      rewrite <- app_comm_cons in H3.
-      eapply scope_duplicate in H3; auto. apply in_app_iff. right.
-      apply in_app_iff. right. apply in_map. auto.
-    - inversion H1. subst. apply IHe0. rewrite app_comm_cons. auto.
-      eapply scope_ext_app. auto.
-  * split; intros. inversion H.
-    simpl. inversion H. 2: inversion H1. subst. constructor.
-    - apply IHe0. auto. auto.
-    - rewrite indexed_to_forall in IHe1.
-      intros. epose (IHe1 i _). destruct a. clear H2 IHe1. Search map nth.
-      replace (ELit 0) with ((varsubst v val) (ELit 0)). rewrite map_nth. apply H5.
-      apply H4. rewrite map_length in H1. auto. auto. reflexivity.
-  * split; intros; inversion H; subst.
-    - simpl. break_match_goal.
-      + apply eqb_eq in Heqb. subst. constructor. apply IHe0_1; eauto.
-        apply scope_duplicate in H5. 2: apply in_or_app; right; constructor; auto.
-        exact H5.
-      + apply eqb_neq in Heqb. constructor.
-        apply IHe0_1; eauto.
-        apply IHe0_2; eauto.
-        eapply scope_ext_app in H0. eauto.
-    - inversion H1.
-  * split; intros. inversion H. subst.
-    simpl. inversion H. 2: inversion H1. subst. break_match_goal.
-    - constructor. rewrite <- app_comm_cons in H3. eapply scope_duplicate.
-      2: exact H3. apply in_list_sound in Heqb. apply in_app_iff. right.
-      apply in_app_iff. right.
-      apply in_map. auto.
-      apply IHe0_2. rewrite <- app_comm_cons in H6. auto.
-      eapply scope_ext_app in H0. eauto.
-    - constructor.
-      apply IHe0_1; eauto. eapply scope_ext_app. eauto.
-      apply IHe0_2; eauto. eapply scope_ext_app. eauto.
-  * split; intros. inversion H. subst. simpl. inversion H. 2: inversion H1. subst.
-    constructor. 
-    eapply IHe0_1; auto. eapply IHe0_2; auto.
-  * split; intros. inversion H. subst. simpl. inversion H. 2: inversion H1. subst.
-    constructor. 
-    eapply IHe0_1; auto. eapply IHe0_2; auto. eapply IHe0_3; auto.
-  * constructor. apply IHe0. apply IHe1.
-  * constructor.
-Unshelve. rewrite map_length in H1. auto.
-Qed.
 
-Theorem scope_funsub v : forall e,
-  (forall Γ, VAL (inr v::Γ) ⊢ e -> forall val, VAL Γ ⊢ val -> VAL Γ ⊢ (funsubst v val e)) /\
-  (forall Γ, EXP (inr v::Γ) ⊢ e -> forall val, EXP Γ ⊢ val -> EXP Γ ⊢ (funsubst v val e)).
-Proof.
-  einduction e using Exp_ind2 with 
-  (Q := fun l => list_forall (fun e => (forall Γ, VAL (inr v::Γ) ⊢ e -> forall val, VAL Γ ⊢ val -> VAL Γ ⊢ (funsubst v val e)) /\
-  (forall Γ, EXP (inr v::Γ) ⊢ e -> forall val, EXP Γ ⊢ val -> EXP Γ ⊢ (funsubst v val e))) l); intros.
-  * split; intros; simpl; constructor. constructor.
-  * split; intros. inversion H.
-    inversion H. 2: inversion H1. simpl. subst. constructor.
-    inversion H2. inversion H1. auto.
-  * split; intros; simpl; break_match_goal; auto. inversion H. constructor.
-    inversion H. 2: inversion H1. subst. apply funid_eqb_neq in Heqb. inversion H2.
-    - inversion H1. subst. congruence.
-    - auto.
-  * split; intros; inversion H; subst; simpl; constructor. 2: constructor.
-    - apply IHe0. rewrite app_comm_cons. auto. apply scope_ext_app. constructor. auto.
-    - inversion H1. subst. apply IHe0. rewrite app_comm_cons. auto.
-      apply scope_ext_app. auto.
-  * split; intros; inversion H; subst; simpl; break_match_goal.
-    - apply funid_eqb_eq in Heqb. subst. constructor. rewrite <- app_comm_cons in H2.
-      eapply scope_duplicate. 2: exact H2.
-      apply in_app_iff. right. apply in_app_iff. left. constructor. auto.
-    - constructor. apply IHe0. rewrite app_comm_cons. auto.
-      apply scope_ext_app. constructor. auto.
-    - inversion H1. subst. apply funid_eqb_eq in Heqb. subst.
-      constructor. constructor. rewrite <- app_comm_cons in H3.
-      eapply scope_duplicate. 2: exact H3.
-      apply in_app_iff. right. apply in_app_iff. left. constructor. auto.
-    - constructor. constructor. inversion H1. subst.
-      apply IHe0. rewrite app_comm_cons. auto.
-      apply scope_ext_app. auto.
-  * split; intros. inversion H.
-    simpl. inversion H. 2: inversion H1. subst. constructor.
-    - apply IHe0. auto. auto.
-    - rewrite indexed_to_forall in IHe1.
-      intros. epose (IHe1 i _). destruct a. clear H2 IHe1. Search map nth.
-      replace (ELit 0) with ((funsubst v val) (ELit 0)). rewrite map_nth. apply H5.
-      apply H4. rewrite map_length in H1. auto. auto. reflexivity.
-  * split; intros; inversion H; subst.
-    - simpl. constructor.
-      apply IHe0_1; eauto.
-      apply IHe0_2; eauto.
-      eapply scope_ext_app in H0. eauto.
-    - inversion H1.
-  * split; intros; inversion H. subst.
-    simpl. break_match_goal.
-    - constructor. apply funid_eqb_eq in Heqb. subst. rewrite <- app_comm_cons in H3.
-      eapply scope_duplicate. 2: exact H3. apply in_app_iff. right.
-      apply in_app_iff. left. constructor. auto.
-      apply funid_eqb_eq in Heqb. subst. rewrite <- app_comm_cons in H6.
-      eapply scope_duplicate. 2: exact H6. apply in_app_iff. intuition.
-    - apply funid_eqb_neq in Heqb. constructor.
-      apply IHe0_1. try rewrite app_comm_cons; eauto.
-      apply scope_ext_app. auto.
-      apply IHe0_2. rewrite app_comm_cons; auto.
-      apply scope_ext_app. auto.
-    - inversion H1.
-  * split; intros. inversion H. subst. simpl. inversion H. 2: inversion H1. subst.
-    constructor. 
-    eapply IHe0_1; auto. eapply IHe0_2; auto.
-  * split; intros. inversion H. subst. simpl. inversion H. 2: inversion H1. subst.
-    constructor. 
-    eapply IHe0_1; auto. eapply IHe0_2; auto. eapply IHe0_3; auto.
-  * constructor. apply IHe0. apply IHe1.
-  * constructor.
-Unshelve. rewrite map_length in H1. auto.
-Qed.
 
-Corollary scope_subst v : forall e,
-  (forall Γ, VAL (v::Γ) ⊢ e -> forall val, VAL Γ ⊢ val -> VAL Γ ⊢ (subst v val e)) /\
-  (forall Γ, EXP (v::Γ) ⊢ e -> forall val, EXP Γ ⊢ val -> EXP Γ ⊢ (subst v val e)).
-Proof.
-  destruct v.
-  - apply scope_sub.
-  - apply scope_funsub.
-Qed.
 
-Lemma element_exist {A : Type} : forall n (l : list A), S n = length l -> exists e l', l = e::l'.
-Proof.
-  intros. destruct l.
-  * inversion H.
-  * apply ex_intro with a. apply ex_intro with l. reflexivity.
-Qed.
 
-Corollary scope_subst_list Γ : forall e,
-  (VAL Γ ⊢ e -> forall vals, length vals = length Γ -> subscoped [] vals -> VALCLOSED (subst_list Γ vals e)) /\
-  (EXP Γ ⊢ e -> forall vals, length vals = length Γ -> subscoped [] vals -> EXPCLOSED (subst_list Γ vals e)).
-Proof.
-  induction Γ; split; intros.
-  * unfold subst_list. simpl. auto.
-  * unfold subst_list. simpl. auto.
-  * unfold subscoped in H1. apply eq_sym, element_exist in H0 as EE. destruct EE, H2.
-    subst. unfold subst_list. simpl.
-    replace (fold_left (fun (acc : Exp) '(v, val) => subst v val acc) (combine Γ x0) (subst a x e)) with (subst_list Γ x0 (subst a x e)). 2: reflexivity.
-    specialize (IHΓ (subst a x e)). destruct IHΓ.
-    inversion H0.
-    epose (H2 _ x0 (eq_sym H5) _). auto.
-  * unfold subscoped in H1. apply eq_sym, element_exist in H0 as EE. destruct EE, H2.
-    subst. unfold subst_list. simpl.
-    replace (fold_left (fun (acc : Exp) '(v, val) => subst v val acc) (combine Γ x0) (subst a x e)) with (subst_list Γ x0 (subst a x e)). 2: reflexivity.
-    specialize (IHΓ (subst a x e)). destruct IHΓ.
-    inversion H0.
-    epose (H3 _ x0 (eq_sym H5) _). auto.
-Unshelve.
-  - apply scope_subst; eauto. specialize (H1 0 (Nat.lt_0_succ _)).
-    simpl in H1. replace Γ with ([] ++ Γ); auto. apply scope_ext_app. auto.
-  - intro. intros. apply (H1 (S i)). simpl. lia.
-  - apply scope_subst; eauto. specialize (H1 0 (Nat.lt_0_succ _)).
-    simpl in H1. replace Γ with ([] ++ Γ); auto. apply scope_ext_app. auto.
-    constructor. auto.
-  - intro. intros. apply (H1 (S i)). simpl. lia.
-Qed.
+
+
 
 (* Lemma VarFunId_eq_dec (v v' : VarFunId) : {v = v'} + {v <> v'}.
 Proof. decide equality. apply string_dec. repeat decide equality. Qed. *)
